trunk/color/Util/Relation/AdjMat.v
@@ -271,15 +271,15 @@ Proof.
 split; intros.
 rewrite Gmorph_iter_le_fast in H; rewrite iter_le_fast_exp2_same in H.
 rewrite iter_le_spec in H; destruct H as [p]; destruct H.
-deduce (iter_tc _ _ _ _ H0); trivial.
-deduce(eq_dec_midex eq_nat_dec).
-deduce (clos_trans_bound_path H0 (@GoM_restricted M)).
+ded (iter_tc _ _ _ _ H0); trivial.
+ded (eq_dec_midex eq_nat_dec).
+ded (clos_trans_bound_path H0 (@GoM_restricted M)).
 rewrite nfirst_length in H1; unfold inclusion in H1.
-deduce (H1 _ _ H); deduce (bound_path_iter_le H2).
+ded (H1 _ _ H); ded (bound_path_iter_le H2).
 rewrite Gmorph_iter_le_fast; rewrite iter_le_fast_spec.
 rewrite iter_le_spec in H3.
 destruct H3 as [p]; exists p. intuition.
-deduce (exp2_log2 dim).
+ded (exp2_log2 dim).
 omega.
 Qed.
 
@@ -388,7 +388,7 @@ Lemma GoM_MoG : forall x y, GoM MoG x y <-> R x y.
 Proof.
 intros. unfold GoM, mat_unbound. split; intros;
 destruct (le_gt_dec dim x); destruct (le_gt_dec dim y);
-try deduce (hyp H);
+try ded (hyp H);
 auto; intuition; try omega; try tauto; try discriminate.
 unfold MoG in H; rewrite mat_build_nth in H.
 destruct (R_dec x y); auto; try discriminate.
