trunk/color/Util/Relation/NotSN.v
@@ -7,7 +7,7 @@ See the COPYRIGHTS and LICENSE files.
 properties of ~SN terms (using classical logic)
 *)
 
-(* $Id: NotSN.v,v 1.1 2007-08-08 09:33:43 blanqui Exp $ *)
+(* $Id: NotSN.v,v 1.2 2008-05-14 12:26:55 blanqui Exp $ *)
 
 Set Implicit Arguments.
 
@@ -22,8 +22,8 @@ Lemma notSN_succ : exists y, R x y /\ ~SN R y.
 
 Proof.
 cut (~(forall y, R x y -> SN R y)).
-intro. deduce (not_forall_imply_exists_not H). destruct H0.
-deduce (imply_to_and _ _ H0). exists x0. auto.
+intro. ded (not_forall_imply_exists_not H). destruct H0.
+ded (imply_to_and _ _ H0). exists x0. auto.
 eapply contraposee_inv. apply SN_intro. exact h.
 Qed.
 
